Translation of modules through Exitify now compiles with Coq (though skipping Exitify.exitifyProgram because of the lack of mutual recursion). Some of the modules are axiomatized though: Id, CoreFVs, CoreUtils, CoreSubst, DynFlags, CoreArity. We can work backwards from Exitify to figure out what functionality we need.

examples/ghc/lib/ConLike.v
@@ -13,12 +13,10 @@ Require Coq.Program.Wf.
 (* Converted imports: *)
 
 Require BasicTypes.
-Require Data.Foldable.
 Require DataCon.
-Require FieldLabel.
 Require GHC.Base.
-Require GHC.List.
 Require Name.
+Require OccName.
 Require PatSyn.
 Require Unique.
 Import GHC.Base.Notations.
@@ -30,10 +28,7 @@ Inductive ConLike : Type
   |  PatSynCon : PatSyn.PatSyn -> ConLike.
 (* Midamble *)
 
-(* nonqualified record selectors*)
-Import FieldLabel.
 
-Instance Unique_ConLike : Unique.Uniquable ConLike := {}. Admitted.
 
 (* Converted value declarations: *)
 
@@ -47,7 +42,20 @@ Local Definition Uniquable__ConLike_getUnique : ConLike -> Unique.Unique :=
 Program Instance Uniquable__ConLike : Unique.Uniquable ConLike :=
   fun _ k => k {| Unique.getUnique__ := Uniquable__ConLike_getUnique |}.
 
-(* Skipping instance NamedThing__ConLike *)
+Local Definition NamedThing__ConLike_getName : ConLike -> Name.Name :=
+  fun arg_0__ =>
+    match arg_0__ with
+    | RealDataCon dc => Name.getName dc
+    | PatSynCon ps => Name.getName ps
+    end.
+
+Local Definition NamedThing__ConLike_getOccName : ConLike -> OccName.OccName :=
+  fun n => Name.nameOccName (NamedThing__ConLike_getName n).
+
+Program Instance NamedThing__ConLike : Name.NamedThing ConLike :=
+  fun _ k =>
+    k {| Name.getName__ := NamedThing__ConLike_getName ;
+         Name.getOccName__ := NamedThing__ConLike_getOccName |}.
 
 (* Skipping instance Outputable__ConLike of class Outputable *)
 
@@ -61,23 +69,6 @@ Definition conLikeArity : ConLike -> BasicTypes.Arity :=
     | RealDataCon data_con => DataCon.dataConSourceArity data_con
     | PatSynCon pat_syn => PatSyn.patSynArity pat_syn
     end.
-
-Definition conLikeFieldLabels : ConLike -> list FieldLabel.FieldLabel :=
-  fun arg_0__ =>
-    match arg_0__ with
-    | RealDataCon data_con => DataCon.dataConFieldLabels data_con
-    | PatSynCon pat_syn => PatSyn.patSynFieldLabels pat_syn
-    end.
-
-Definition conLikesWithFields
-   : list ConLike -> list FieldLabel.FieldLabelString -> list ConLike :=
-  fun con_likes lbls =>
-    let has_fld :=
-      fun dc lbl =>
-        Data.Foldable.any (fun fl => FieldLabel.flLabel fl GHC.Base.== lbl)
-        (conLikeFieldLabels dc) in
-    let has_flds := fun dc => Data.Foldable.all (has_fld dc) lbls in
-    GHC.List.filter has_flds con_likes.
 
 Definition conLikeName : ConLike -> Name.Name :=
   fun arg_0__ =>
@@ -101,11 +92,10 @@ Program Instance Eq___ConLike : GHC.Base.Eq_ ConLike :=
          GHC.Base.op_zsze____ := Eq___ConLike_op_zsze__ |}.
 
 (* External variables:
-     bool list negb BasicTypes.Arity Data.Foldable.all Data.Foldable.any
-     DataCon.DataCon DataCon.dataConFieldLabels DataCon.dataConName
-     DataCon.dataConSourceArity FieldLabel.FieldLabel FieldLabel.FieldLabelString
-     FieldLabel.flLabel GHC.Base.Eq_ GHC.Base.op_zeze__ GHC.Base.op_zeze____
-     GHC.Base.op_zsze____ GHC.List.filter Name.Name PatSyn.PatSyn PatSyn.patSynArity
-     PatSyn.patSynFieldLabels PatSyn.patSynName Unique.Uniquable Unique.Unique
+     bool negb BasicTypes.Arity DataCon.DataCon DataCon.dataConName
+     DataCon.dataConSourceArity GHC.Base.Eq_ GHC.Base.op_zeze__ GHC.Base.op_zeze____
+     GHC.Base.op_zsze____ Name.Name Name.NamedThing Name.getName Name.getName__
+     Name.getOccName__ Name.nameOccName OccName.OccName PatSyn.PatSyn
+     PatSyn.patSynArity PatSyn.patSynName Unique.Uniquable Unique.Unique
      Unique.getUnique Unique.getUnique__
 *)
