examples/ghc/lib/CoreFVs.v
@@ -12,32 +12,17 @@ Require Coq.Program.Wf.
 
 (* Preamble *)
 
-
+Require Import CoreSyn.
 
 (* Converted imports: *)
 
 Require BasicTypes.
 Require CoreSyn.
-Require Data.Foldable.
-Require Data.Tuple.
 Require FV.
-Require GHC.Base.
-Require GHC.List.
-Require GHC.Num.
-Require Id.
-Require IdInfo.
-Require Maybes.
-Require Name.
 Require NameSet.
-Require Panic.
 Require TyCon.
-Require UniqSet.
-Require Unique.
-Require Util.
 Require Var.
 Require VarSet.
-Import GHC.Base.Notations.
-Import GHC.Num.Notations.
 
 (* Converted type declarations: *)
 
@@ -57,422 +42,170 @@ Definition CoreAltWithFVs :=
   (AnnAlt Var.Id FVAnn)%type.
 (* Midamble *)
 
-Require Import Var.
 
-Parameter tickish_fvs : CoreSyn.Tickish Var.Id -> FV.FV.
-
-(* Very bad treatment of guards. Plus needs a lot from Coercion/Type/TyCoRep *)
-Parameter freeVars : CoreSyn.CoreExpr -> CoreExprWithFVs.
-Parameter expr_fvs : CoreSyn.CoreExpr -> FV.FV.
-
-Parameter exprOrphNames : CoreSyn.CoreExpr -> NameSet.NameSet.
-(*
-Fixpoint exprOrphNames (e : CoreSyn.CoreExpr) : NameSet.NameSet :=
-    let go_alt :=
-      fun arg_13__ => match arg_13__ with | pair (pair _ _) r => exprOrphNames r end in
-    let exprsOrphNames : list CoreSyn.CoreExpr -> NameSet.NameSet :=
-        fun es =>
-          Data.Foldable.foldr (NameSet.unionNameSet GHC.Base.∘ exprOrphNames)
-                              NameSet.emptyNameSet es in
-    match e with
-    | CoreSyn.Var v => let n := Id.idName v in
-                      if Name.isExternalName n : bool
-                      then NameSet.unitNameSet n
-                      else NameSet.emptyNameSet
-    | CoreSyn.Lit _ => NameSet.emptyNameSet
-    | CoreSyn.Type_ ty => orphNamesOfType ty
-    | CoreSyn.Coercion co => orphNamesOfCo co
-    | CoreSyn.App e1 e2 => NameSet.unionNameSet (exprOrphNames e1) (exprOrphNames e2)
-    | CoreSyn.Lam v e => NameSet.delFromNameSet (exprOrphNames e) (Id.idName v)
-    | CoreSyn.Tick _ e => exprOrphNames e
-    | CoreSyn.Cast e co => NameSet.unionNameSet (exprOrphNames e) (orphNamesOfCo co)
-    | CoreSyn.Let (CoreSyn.NonRec _ r) e => NameSet.unionNameSet (exprOrphNames e) (exprOrphNames r)
-    | CoreSyn.Let (CoreSyn.Rec prs) e => (exprOrphNames e)
-(*      NameSet.unionNameSet (exprsOrphNames
-                              (GHC.Base.map Data.Tuple.snd prs))  *)
-    | CoreSyn.Case e _ ty as_ => NameSet.unionNameSet
-                                  (NameSet.unionNameSet (exprOrphNames e)
-                                                        (orphNamesOfType ty))
-                                  (NameSet.unionNameSets (GHC.Base.map go_alt as_))
-    end. *)
-
-Parameter orphNamesOfCo : Core.Coercion -> NameSet.NameSet.
-(*
-Fixpoint orphNamesOfCo (arg_0__ : Core.Coercion): NameSet.NameSet :=
-  let  orphNamesOfCos : list Core.Coercion -> NameSet.NameSet :=
-       orphNamesOfThings orphNamesOfCo in
-  let orphNamesOfProv : Core.UnivCoProvenance -> NameSet.NameSet :=
-  fun arg_0__ =>
-    match arg_0__ with
-      | Core.UnsafeCoerceProv => NameSet.emptyNameSet
-      | Core.PhantomProv co => orphNamesOfCo co
-      | Core.ProofIrrelProv co => orphNamesOfCo co
-      | Core.PluginProv _ => NameSet.emptyNameSet
-      | Core.HoleProv _ => NameSet.emptyNameSet
-    end in
-
-  match arg_0__ with
-             | Core.Refl _ ty => orphNamesOfType ty
-             | Core.TyConAppCo _ tc cos => NameSet.unionNameSet (NameSet.unitNameSet
-                                                                (Name.getName tc)) (orphNamesOfCos cos)
-             | Core.AppCo co1 co2 => NameSet.unionNameSet (orphNamesOfCo co1) (orphNamesOfCo
-                                                          co2)
-             | Core.ForAllCo _ kind_co co => NameSet.unionNameSet (orphNamesOfCo kind_co)
-                                                                  (orphNamesOfCo co)
-             | Core.CoVarCo _ => NameSet.emptyNameSet
-             | Core.AxiomInstCo con _ cos => NameSet.unionNameSet (orphNamesOfCoCon con)
-                                                                  (orphNamesOfCos cos)
-             | Core.UnivCo p _ t1 t2 => NameSet.unionNameSet (NameSet.unionNameSet
-                                                             (orphNamesOfProv p) (orphNamesOfType t1)) (orphNamesOfType
-                                                             t2)
-             | Core.SymCo co => orphNamesOfCo co
-             | Core.TransCo co1 co2 => NameSet.unionNameSet (orphNamesOfCo co1)
-                                                            (orphNamesOfCo co2)
-             | Core.NthCo _ co => orphNamesOfCo co
-             | Core.LRCo _ co => orphNamesOfCo co
-             | Core.InstCo co arg => NameSet.unionNameSet (orphNamesOfCo co) (orphNamesOfCo
-                                                          arg)
-             | Core.CoherenceCo co1 co2 => NameSet.unionNameSet (orphNamesOfCo co1)
-                                                                (orphNamesOfCo co2)
-             | Core.KindCo co => orphNamesOfCo co
-             | Core.SubCo co => orphNamesOfCo co
-             | Core.AxiomRuleCo _ cs => orphNamesOfCos cs
-           end.
-*)
 (* Converted value declarations: *)
 
-Definition aFreeVar : Var.Var -> VarSet.DVarSet :=
-  VarSet.unitDVarSet.
+Axiom exprFreeVars : CoreSyn.CoreExpr -> VarSet.VarSet.
 
-Definition exprFVs : CoreSyn.CoreExpr -> FV.FV :=
-  FV.filterFV Var.isLocalVar GHC.Base.∘ expr_fvs.
+Axiom exprsFreeVarsList : list CoreSyn.CoreExpr -> list Var.Var.
 
-Definition exprFreeVars : CoreSyn.CoreExpr -> VarSet.VarSet :=
-  FV.fvVarSet GHC.Base.∘ exprFVs.
+Axiom exprsFreeVars : list CoreSyn.CoreExpr -> VarSet.VarSet.
 
-Definition exprFreeVarsDSet : CoreSyn.CoreExpr -> VarSet.DVarSet :=
-  FV.fvDVarSet GHC.Base.∘ exprFVs.
+Axiom exprsFVs : list CoreSyn.CoreExpr -> FV.FV.
 
-Definition exprFreeVarsList : CoreSyn.CoreExpr -> list Var.Var :=
-  FV.fvVarList GHC.Base.∘ exprFVs.
+Axiom exprFreeVarsList : CoreSyn.CoreExpr -> list Var.Var.
 
-Definition exprsFVs : list CoreSyn.CoreExpr -> FV.FV :=
-  fun exprs => FV.mapUnionFV exprFVs exprs.
+Axiom exprFreeVarsDSet : CoreSyn.CoreExpr -> VarSet.DVarSet.
 
-Definition exprsFreeVars : list CoreSyn.CoreExpr -> VarSet.VarSet :=
-  FV.fvVarSet GHC.Base.∘ exprsFVs.
+Axiom exprFVs : CoreSyn.CoreExpr -> FV.FV.
 
-Definition exprsFreeVarsList : list CoreSyn.CoreExpr -> list Var.Var :=
-  FV.fvVarList GHC.Base.∘ exprsFVs.
+Axiom exprFreeIds : CoreSyn.CoreExpr -> VarSet.IdSet.
 
-Definition exprSomeFreeVars
-   : FV.InterestingVarFun -> CoreSyn.CoreExpr -> VarSet.VarSet :=
-  fun fv_cand e => FV.fvVarSet (FV.filterFV fv_cand (expr_fvs e)).
+Axiom exprFreeIdsDSet : CoreSyn.CoreExpr -> VarSet.DIdSet.
 
-Definition exprFreeIds : CoreSyn.CoreExpr -> VarSet.IdSet :=
-  exprSomeFreeVars Var.isLocalId.
+Axiom exprFreeIdsList : CoreSyn.CoreExpr -> list Var.Id.
 
-Definition exprSomeFreeVarsDSet
-   : FV.InterestingVarFun -> CoreSyn.CoreExpr -> VarSet.DVarSet :=
-  fun fv_cand e => FV.fvDVarSet (FV.filterFV fv_cand (expr_fvs e)).
+Axiom exprsFreeIdsDSet : list CoreSyn.CoreExpr -> VarSet.DIdSet.
 
-Definition exprFreeIdsDSet : CoreSyn.CoreExpr -> VarSet.DIdSet :=
-  exprSomeFreeVarsDSet Var.isLocalId.
+Axiom exprsFreeIdsList : list CoreSyn.CoreExpr -> list Var.Id.
 
-Definition exprSomeFreeVarsList
-   : FV.InterestingVarFun -> CoreSyn.CoreExpr -> list Var.Var :=
-  fun fv_cand e => FV.fvVarList (FV.filterFV fv_cand (expr_fvs e)).
+Axiom bindFreeVars : CoreSyn.CoreBind -> VarSet.VarSet.
 
-Definition exprFreeIdsList : CoreSyn.CoreExpr -> list Var.Id :=
-  exprSomeFreeVarsList Var.isLocalId.
+Axiom exprSomeFreeVars : FV.InterestingVarFun ->
+                         CoreSyn.CoreExpr -> VarSet.VarSet.
 
-Definition exprsOrphNames : list CoreSyn.CoreExpr -> NameSet.NameSet :=
-  fun es =>
-    Data.Foldable.foldr (NameSet.unionNameSet GHC.Base.∘ exprOrphNames)
-    NameSet.emptyNameSet es.
+Axiom exprSomeFreeVarsList : FV.InterestingVarFun ->
+                             CoreSyn.CoreExpr -> list Var.Var.
 
-Definition exprsSomeFreeVars
-   : FV.InterestingVarFun -> list CoreSyn.CoreExpr -> VarSet.VarSet :=
-  fun fv_cand es => FV.fvVarSet (FV.filterFV fv_cand (FV.mapUnionFV expr_fvs es)).
+Axiom exprSomeFreeVarsDSet : FV.InterestingVarFun ->
+                             CoreSyn.CoreExpr -> VarSet.DVarSet.
 
-Definition exprsSomeFreeVarsDSet
-   : FV.InterestingVarFun -> list CoreSyn.CoreExpr -> VarSet.DVarSet :=
-  fun fv_cand e => FV.fvDVarSet (FV.filterFV fv_cand (FV.mapUnionFV expr_fvs e)).
+Axiom exprsSomeFreeVars : FV.InterestingVarFun ->
+                          list CoreSyn.CoreExpr -> VarSet.VarSet.
 
-Definition exprsFreeIdsDSet : list CoreSyn.CoreExpr -> VarSet.DIdSet :=
-  exprsSomeFreeVarsDSet Var.isLocalId.
+Axiom exprsSomeFreeVarsList : FV.InterestingVarFun ->
+                              list CoreSyn.CoreExpr -> list Var.Var.
 
-Definition exprsSomeFreeVarsList
-   : FV.InterestingVarFun -> list CoreSyn.CoreExpr -> list Var.Var :=
-  fun fv_cand es =>
-    FV.fvVarList (FV.filterFV fv_cand (FV.mapUnionFV expr_fvs es)).
+Axiom exprsSomeFreeVarsDSet : FV.InterestingVarFun ->
+                              list CoreSyn.CoreExpr -> VarSet.DVarSet.
 
-Definition exprsFreeIdsList : list CoreSyn.CoreExpr -> list Var.Id :=
-  exprsSomeFreeVarsList Var.isLocalId.
+Axiom stableUnfoldingVars : CoreSyn.Unfolding -> option VarSet.VarSet.
 
-Definition exprs_fvs : list CoreSyn.CoreExpr -> FV.FV :=
-  fun exprs => FV.mapUnionFV expr_fvs exprs.
+Axiom idUnfoldingVars : Var.Id -> VarSet.VarSet.
 
-Definition stableUnfoldingFVs : CoreSyn.Unfolding -> option FV.FV :=
-  fun unf =>
-    let j_1__ :=
-      match unf with
-      | CoreSyn.DFunUnfolding bndrs _ args =>
-          Some (FV.filterFV Var.isLocalVar (FV.delFVs (VarSet.mkVarSet bndrs) (exprs_fvs
-                                                       args)))
-      | _other => None
-      end in
-    match unf with
-    | CoreSyn.CoreUnfolding rhs src _ _ _ _ _ _ =>
-        if CoreSyn.isStableSource src : bool
-        then Some (FV.filterFV Var.isLocalVar (expr_fvs rhs)) else
-        j_1__
-    | _ => j_1__
-    end.
+Axiom freeVars : CoreSyn.CoreExpr -> CoreExprWithFVs.
 
-Definition idUnfoldingFVs : Var.Id -> FV.FV :=
-  fun id => Maybes.orElse (stableUnfoldingFVs (Id.realIdUnfolding id)) FV.emptyFV.
+Axiom freeVarsBind : CoreSyn.CoreBind ->
+                     VarSet.DVarSet -> (CoreBindWithFVs * VarSet.DVarSet)%type.
 
-Definition idUnfoldingVars : Var.Id -> VarSet.VarSet :=
-  fun id => FV.fvVarSet (idUnfoldingFVs id).
+Axiom bndrRuleAndUnfoldingVarsDSet : Var.Id -> VarSet.DVarSet.
 
-Definition stableUnfoldingVars : CoreSyn.Unfolding -> option VarSet.VarSet :=
-  fun unf => GHC.Base.fmap FV.fvVarSet (stableUnfoldingFVs unf).
+Axiom dIdFreeVars : Var.Id -> VarSet.DVarSet.
 
-Definition freeVarsOf : CoreExprWithFVs -> VarSet.DIdSet :=
-  fun arg_0__ => let 'pair fvs _ := arg_0__ in fvs.
+Axiom idFreeVars : Var.Id -> VarSet.VarSet.
 
-Definition freeVarsOfAnn : FVAnn -> VarSet.DIdSet :=
-  fun fvs => fvs.
+Axiom idFVs : Var.Id -> FV.FV.
 
-Definition idRuleFVs : Var.Id -> FV.FV :=
-  fun id =>
-    if andb Util.debugIsOn (negb (Var.isId id)) : bool
-    then (Panic.assertPanic (GHC.Base.hs_string__ "ghc/compiler/coreSyn/CoreFVs.hs")
-          #645)
-    else FV.mkFVs (VarSet.dVarSetElems (IdInfo.ruleInfoFreeVars (Id.idSpecialisation
-                                                                 id))).
+Axiom vectsFreeVars : list CoreSyn.CoreVect -> VarSet.VarSet.
 
-Definition idRuleVars : Var.Id -> VarSet.VarSet :=
-  fun id => FV.fvVarSet (idRuleFVs id).
+Axiom idRuleRhsVars : (BasicTypes.Activation -> bool) ->
+                      Var.Id -> VarSet.VarSet.
 
-Definition bndrRuleAndUnfoldingFVs : Var.Id -> FV.FV :=
-  fun id =>
-    if Var.isId id : bool then FV.unionFV (idRuleFVs id) (idUnfoldingFVs id) else
-    FV.emptyFV.
+Axiom ruleRhsFreeVars : CoreSyn.CoreRule -> VarSet.VarSet.
 
-Definition bndrRuleAndUnfoldingVarsDSet : Var.Id -> VarSet.DVarSet :=
-  fun id => FV.fvDVarSet (bndrRuleAndUnfoldingFVs id).
+Axiom ruleLhsFreeIdsList : CoreSyn.CoreRule -> list Var.Var.
 
-Definition rhs_fvs : (Var.Id * CoreSyn.CoreExpr)%type -> FV.FV :=
-  fun arg_0__ =>
-    let 'pair bndr rhs := arg_0__ in
-    FV.unionFV (expr_fvs rhs) (bndrRuleAndUnfoldingFVs bndr).
+Axiom ruleLhsFreeIds : CoreSyn.CoreRule -> VarSet.VarSet.
 
-Definition noFVs : VarSet.VarSet :=
-  VarSet.emptyVarSet.
+Axiom ruleLhsFVIds : CoreSyn.CoreRule -> FV.FV.
 
-Definition vectsFreeVars : list CoreSyn.CoreVect -> VarSet.VarSet :=
-  let vectFreeVars :=
-    fun arg_0__ =>
-      match arg_0__ with
-      | CoreSyn.Vect _ rhs => FV.fvVarSet (FV.filterFV Var.isLocalId (expr_fvs rhs))
-      | CoreSyn.NoVect _ => noFVs
-      | CoreSyn.VectType _ _ _ => noFVs
-      | CoreSyn.VectClass _ => noFVs
-      | CoreSyn.VectInst _ => noFVs
-      end in
-  VarSet.mapUnionVarSet vectFreeVars.
+Axiom rulesFreeVarsDSet : list CoreSyn.CoreRule -> VarSet.DVarSet.
 
-Definition orphNamesOfCoAxBranches {br}
-   : CoAxiom.Branches br -> NameSet.NameSet :=
-  Data.Foldable.foldr (NameSet.unionNameSet GHC.Base.∘ orphNamesOfCoAxBranch)
-  NameSet.emptyNameSet GHC.Base.∘
-  CoAxiom.fromBranches.
+Axiom rulesFVs : list CoreSyn.CoreRule -> FV.FV.
 
-Definition orphNamesOfThings {a}
-   : (a -> NameSet.NameSet) -> list a -> NameSet.NameSet :=
-  fun f =>
-    Data.Foldable.foldr (NameSet.unionNameSet GHC.Base.∘ f) NameSet.emptyNameSet.
+Axiom rulesFreeVars : list CoreSyn.CoreRule -> VarSet.VarSet.
 
-Definition orphNamesOfTypes : list unit -> NameSet.NameSet :=
-  orphNamesOfThings orphNamesOfType.
+Axiom ruleFreeVars : CoreSyn.CoreRule -> VarSet.VarSet.
 
-Definition orphNamesOfAxiom {br} : list br -> NameSet.NameSet :=
-  fun axiom =>
-    NameSet.extendNameSet (orphNamesOfTypes (Data.Foldable.concatMap
-                                             CoAxiom.coAxBranchLHS (CoAxiom.fromBranches (CoAxiom.coAxiomBranches
-                                                                                          axiom)))) (Name.getName
-                           (CoAxiom.coAxiomTyCon axiom)).
+Axiom ruleFVs : CoreSyn.CoreRule -> FV.FV.
 
-Definition orphNamesOfCos : list unit -> NameSet.NameSet :=
-  orphNamesOfThings orphNamesOfCo.
+Axiom exprs_fvs : list CoreSyn.CoreExpr -> FV.FV.
 
-Definition orphNamesOfTyCon : TyCon.TyCon -> NameSet.NameSet :=
-  fun tycon =>
-    NameSet.unionNameSet (NameSet.unitNameSet (Name.getName tycon))
-                         (match TyCon.tyConClass_maybe tycon with
-                          | None => NameSet.emptyNameSet
-                          | Some cls => NameSet.unitNameSet (Name.getName cls)
-                          end).
+Axiom stableUnfoldingFVs : CoreSyn.Unfolding -> option FV.FV.
 
-Definition unionFVs : VarSet.DVarSet -> VarSet.DVarSet -> VarSet.DVarSet :=
-  VarSet.unionDVarSet.
+Axiom idUnfoldingFVs : Var.Id -> FV.FV.
 
-Definition unionFVss : list VarSet.DVarSet -> VarSet.DVarSet :=
-  VarSet.unionDVarSets.
+Axiom bndrRuleAndUnfoldingFVs : Var.Id -> FV.FV.
 
-Definition varTypeTyCoFVs : Var.Var -> FV.FV :=
-  fun var => TyCoRep.tyCoFVsOfType (Var.varType var).
+Axiom rhs_fvs : (Var.Id * CoreSyn.CoreExpr)%type -> FV.FV.
 
-Definition varTypeTyCoVars : Var.Var -> VarSet.TyCoVarSet :=
-  fun var => FV.fvVarSet (varTypeTyCoFVs var).
+Axiom expr_fvs : CoreSyn.CoreExpr -> FV.FV.
 
-Definition dVarTypeTyCoVars : Var.Var -> VarSet.DTyCoVarSet :=
-  fun var => FV.fvDVarSet (varTypeTyCoFVs var).
+Axiom addBndrs : list CoreSyn.CoreBndr -> FV.FV -> FV.FV.
 
-Definition delBinderFV : Var.Var -> VarSet.DVarSet -> VarSet.DVarSet :=
-  fun b s => unionFVs (VarSet.delDVarSet s b) (dVarTypeTyCoVars b).
+Axiom addBndr : CoreSyn.CoreBndr -> FV.FV -> FV.FV.
 
-Definition delBindersFV : list Var.Var -> VarSet.DVarSet -> VarSet.DVarSet :=
-  fun bs fvs => Data.Foldable.foldr delBinderFV fvs bs.
+(* tickish_fvs skipped *)
 
-Definition freeVarsBind
-   : CoreSyn.CoreBind ->
-     VarSet.DVarSet -> (CoreBindWithFVs * VarSet.DVarSet)%type :=
-  fun arg_0__ arg_1__ =>
-    match arg_0__, arg_1__ with
-    | CoreSyn.NonRec binder rhs, body_fvs =>
-        let body_fvs2 := delBinderFV binder body_fvs in
-        let rhs2 := freeVars rhs in
-        pair (CoreSyn.AnnNonRec binder rhs2) (unionFVs (unionFVs (freeVarsOf rhs2)
-                                                                 body_fvs2) (bndrRuleAndUnfoldingVarsDSet binder))
-    | CoreSyn.Rec binds, body_fvs =>
-        let 'pair binders rhss := GHC.List.unzip binds in
-        let rhss2 := GHC.Base.map freeVars rhss in
-        let rhs_body_fvs :=
-          Data.Foldable.foldr (unionFVs GHC.Base.∘ freeVarsOf) body_fvs rhss2 in
-        let binders_fvs :=
-          FV.fvDVarSet (FV.mapUnionFV bndrRuleAndUnfoldingFVs binders) in
-        let all_fvs := unionFVs rhs_body_fvs binders_fvs in
-        pair (CoreSyn.AnnRec (GHC.List.zip binders rhss2)) (delBindersFV binders
-              all_fvs)
-    end.
+Axiom exprsOrphNames : list CoreSyn.CoreExpr -> NameSet.NameSet.
 
-Definition idFVs : Var.Id -> FV.FV :=
-  fun id =>
-    if andb Util.debugIsOn (negb (Var.isId id)) : bool
-    then (Panic.assertPanic (GHC.Base.hs_string__ "ghc/compiler/coreSyn/CoreFVs.hs")
-          #629)
-    else FV.unionFV (varTypeTyCoFVs id) (bndrRuleAndUnfoldingFVs id).
+(* exprOrphNames skipped *)
 
-Definition dIdFreeVars : Var.Id -> VarSet.DVarSet :=
-  fun id => FV.fvDVarSet (idFVs id).
+(* orphNamesOfFamInst skipped *)
 
-Definition idFreeVars : Var.Id -> VarSet.VarSet :=
-  fun id =>
-    if andb Util.debugIsOn (negb (Var.isId id)) : bool
-    then (Panic.assertPanic (GHC.Base.hs_string__ "ghc/compiler/coreSyn/CoreFVs.hs")
-          #622)
-    else FV.fvVarSet (idFVs id).
+Axiom orphNamesOfAxiom : forall {br}, list br -> NameSet.NameSet.
 
-Definition addBndr : CoreSyn.CoreBndr -> FV.FV -> FV.FV :=
-  fun bndr fv fv_cand in_scope acc =>
-    (FV.unionFV (varTypeTyCoFVs bndr) (FV.delFV bndr fv)) fv_cand in_scope acc.
+Axiom orphNamesOfCos : list unit -> NameSet.NameSet.
 
-Definition addBndrs : list CoreSyn.CoreBndr -> FV.FV -> FV.FV :=
-  fun bndrs fv => Data.Foldable.foldr addBndr fv bndrs.
+(* orphNamesOfProv skipped *)
 
-Definition bindFreeVars : CoreSyn.CoreBind -> VarSet.VarSet :=
-  fun arg_0__ =>
-    match arg_0__ with
-    | CoreSyn.NonRec b r =>
-        FV.fvVarSet (FV.filterFV Var.isLocalVar (rhs_fvs (pair b r)))
-    | CoreSyn.Rec prs =>
-        FV.fvVarSet (FV.filterFV Var.isLocalVar (addBndrs (GHC.Base.map Data.Tuple.fst
-                                                           prs) (FV.mapUnionFV rhs_fvs prs)))
-    end.
+(* orphNamesOfCo skipped *)
 
-Definition idRuleRhsVars
-   : (BasicTypes.Activation -> bool) -> Var.Id -> VarSet.VarSet :=
-  fun is_active id =>
-    let get_fvs :=
-      fun arg_0__ =>
-        match arg_0__ with
-        | CoreSyn.Rule _ act fn _ bndrs _ rhs _ _ _ _ =>
-            let fvs :=
-              FV.fvVarSet (FV.filterFV Var.isLocalVar (addBndrs bndrs (expr_fvs rhs))) in
-            if is_active act : bool
-            then UniqSet.delOneFromUniqSet_Directly fvs (Unique.getUnique fn) else
-            noFVs
-        | _ => noFVs
-        end in
-    VarSet.mapUnionVarSet get_fvs (Id.idCoreRules id).
+Axiom orphNamesOfTypes : list unit -> NameSet.NameSet.
 
-Definition ruleFVs : CoreSyn.CoreRule -> FV.FV :=
-  fun arg_0__ =>
-    match arg_0__ with
-    | CoreSyn.BuiltinRule _ _ _ _ => FV.emptyFV
-    | CoreSyn.Rule _ _ _do_not_include _ bndrs args rhs _ _ _ _ =>
-        FV.filterFV Var.isLocalVar (addBndrs bndrs (exprs_fvs (cons rhs args)))
-    end.
+(* orphNamesOfType skipped *)
 
-Definition ruleFreeVars : CoreSyn.CoreRule -> VarSet.VarSet :=
-  FV.fvVarSet GHC.Base.∘ ruleFVs.
+(* orphNamesOfCoAxBranch skipped *)
 
-Definition rulesFreeVars : list CoreSyn.CoreRule -> VarSet.VarSet :=
-  fun rules => VarSet.mapUnionVarSet ruleFreeVars rules.
+(* orphNamesOfCoAxBranches skipped *)
 
-Definition rulesFVs : list CoreSyn.CoreRule -> FV.FV :=
-  FV.mapUnionFV ruleFVs.
+(* orphNamesOfCoCon skipped *)
 
-Definition rulesFreeVarsDSet : list CoreSyn.CoreRule -> VarSet.DVarSet :=
-  fun rules => FV.fvDVarSet (rulesFVs rules).
+Axiom orphNamesOfTyCon : TyCon.TyCon -> NameSet.NameSet.
 
-Definition ruleLhsFVIds : CoreSyn.CoreRule -> FV.FV :=
-  fun arg_0__ =>
-    match arg_0__ with
-    | CoreSyn.BuiltinRule _ _ _ _ => FV.emptyFV
-    | CoreSyn.Rule _ _ _ _ bndrs args _ _ _ _ _ =>
-        FV.filterFV Var.isLocalId (addBndrs bndrs (exprs_fvs args))
-    end.
+Axiom orphNamesOfThings : forall {a},
+                          (a -> NameSet.NameSet) -> list a -> NameSet.NameSet.
 
-Definition ruleLhsFreeIds : CoreSyn.CoreRule -> VarSet.VarSet :=
-  FV.fvVarSet GHC.Base.∘ ruleLhsFVIds.
+Axiom freeVarsOf : CoreExprWithFVs -> VarSet.DIdSet.
 
-Definition ruleLhsFreeIdsList : CoreSyn.CoreRule -> list Var.Var :=
-  FV.fvVarList GHC.Base.∘ ruleLhsFVIds.
+Axiom freeVarsOfAnn : FVAnn -> VarSet.DIdSet.
 
-Definition ruleRhsFreeVars : CoreSyn.CoreRule -> VarSet.VarSet :=
-  fun arg_0__ =>
-    match arg_0__ with
-    | CoreSyn.BuiltinRule _ _ _ _ => noFVs
-    | CoreSyn.Rule _ _ _ _ bndrs _ rhs _ _ _ _ =>
-        FV.fvVarSet (FV.filterFV Var.isLocalVar (addBndrs bndrs (expr_fvs rhs)))
-    end.
+Axiom noFVs : VarSet.VarSet.
+
+Axiom aFreeVar : Var.Var -> VarSet.DVarSet.
+
+Axiom delBindersFV : list Var.Var -> VarSet.DVarSet -> VarSet.DVarSet.
+
+Axiom delBinderFV : Var.Var -> VarSet.DVarSet -> VarSet.DVarSet.
+
+Axiom unionFVs : VarSet.DVarSet -> VarSet.DVarSet -> VarSet.DVarSet.
+
+Axiom unionFVss : list VarSet.DVarSet -> VarSet.DVarSet.
+
+Axiom varTypeTyCoVars : Var.Var -> VarSet.TyCoVarSet.
+
+Axiom dVarTypeTyCoVars : Var.Var -> VarSet.DTyCoVarSet.
+
+Axiom varTypeTyCoFVs : Var.Var -> FV.FV.
+
+Axiom idRuleVars : Var.Id -> VarSet.VarSet.
+
+Axiom idRuleFVs : Var.Id -> FV.FV.
 
 (* External variables:
-     AnnAlt AnnExpr None Some andb bool cons exprOrphNames expr_fvs freeVars list
-     negb op_zt__ option orphNamesOfCo orphNamesOfCoAxBranch orphNamesOfType pair
-     unit BasicTypes.Activation CoAxiom.Branches CoAxiom.coAxBranchLHS
-     CoAxiom.coAxiomBranches CoAxiom.coAxiomTyCon CoAxiom.fromBranches
-     CoreSyn.AnnBind CoreSyn.AnnExpr' CoreSyn.AnnNonRec CoreSyn.AnnRec
-     CoreSyn.BuiltinRule CoreSyn.CoreBind CoreSyn.CoreBndr CoreSyn.CoreExpr
-     CoreSyn.CoreRule CoreSyn.CoreUnfolding CoreSyn.CoreVect CoreSyn.DFunUnfolding
-     CoreSyn.NoVect CoreSyn.NonRec CoreSyn.Rec CoreSyn.Rule CoreSyn.Unfolding
-     CoreSyn.Vect CoreSyn.VectClass CoreSyn.VectInst CoreSyn.VectType
-     CoreSyn.isStableSource Data.Foldable.concatMap Data.Foldable.foldr
-     Data.Tuple.fst FV.FV FV.InterestingVarFun FV.delFV FV.delFVs FV.emptyFV
-     FV.filterFV FV.fvDVarSet FV.fvVarList FV.fvVarSet FV.mapUnionFV FV.mkFVs
-     FV.unionFV GHC.Base.fmap GHC.Base.map GHC.Base.op_z2218U__ GHC.List.unzip
-     GHC.List.zip GHC.Num.fromInteger Id.idCoreRules Id.idSpecialisation
-     Id.realIdUnfolding IdInfo.ruleInfoFreeVars Maybes.orElse Name.getName
-     NameSet.NameSet NameSet.emptyNameSet NameSet.extendNameSet NameSet.unionNameSet
-     NameSet.unitNameSet Panic.assertPanic TyCoRep.tyCoFVsOfType TyCon.TyCon
-     TyCon.tyConClass_maybe UniqSet.delOneFromUniqSet_Directly Unique.getUnique
-     Util.debugIsOn Var.Id Var.Var Var.isId Var.isLocalId Var.isLocalVar Var.varType
-     VarSet.DIdSet VarSet.DTyCoVarSet VarSet.DVarSet VarSet.IdSet VarSet.TyCoVarSet
-     VarSet.VarSet VarSet.dVarSetElems VarSet.delDVarSet VarSet.emptyVarSet
-     VarSet.mapUnionVarSet VarSet.mkVarSet VarSet.unionDVarSet VarSet.unionDVarSets
-     VarSet.unitDVarSet
+     AnnAlt AnnExpr bool list op_zt__ option unit BasicTypes.Activation
+     CoreSyn.AnnBind CoreSyn.AnnExpr' CoreSyn.CoreBind CoreSyn.CoreBndr
+     CoreSyn.CoreExpr CoreSyn.CoreRule CoreSyn.CoreVect CoreSyn.Unfolding FV.FV
+     FV.InterestingVarFun NameSet.NameSet TyCon.TyCon Var.Id Var.Var VarSet.DIdSet
+     VarSet.DTyCoVarSet VarSet.DVarSet VarSet.IdSet VarSet.TyCoVarSet VarSet.VarSet
 *)
