examples/ghc/lib/Exitify.v
@@ -16,15 +16,16 @@ Require BasicTypes.
 Require Coq.Init.Datatypes.
 Require CoreFVs.
 Require CoreSyn.
-Require CoreUtils.
 Require Data.Bifunctor.
 Require Data.Foldable.
 Require Data.Traversable.
 Require Data.Tuple.
 Require FastString.
 Require GHC.Base.
+Require GHC.DeferredFix.
 Require GHC.List.
 Require Id.
+Require Panic.
 Require State.
 Require Unique.
 Require Var.
@@ -73,203 +74,162 @@ Definition exitify
      : list Var.Var ->
        CoreFVs.CoreExprWithFVs ->
        State.State (list (Var.Id * CoreSyn.CoreExpr)%type) CoreSyn.CoreExpr :=
-      fix go arg_1__ arg_2__
-            := match arg_1__, arg_2__ with
-               | captured, ann_e =>
-                   let j_4__ :=
-                     match arg_1__, arg_2__ with
-                     | _, ann_e => GHC.Base.return_ (CoreSyn.deAnnotate ann_e)
-                     end in
-                   let j_22__ :=
-                     match arg_1__, arg_2__ with
-                     | captured, pair _ (CoreSyn.AnnCase scrut bndr ty alts) =>
-                         Data.Traversable.forM alts (fun arg_5__ =>
-                                                       let 'pair (pair dc pats) rhs := arg_5__ in
-                                                       go (Coq.Init.Datatypes.app captured (Coq.Init.Datatypes.app (cons
-                                                                                                                    bndr
-                                                                                                                    nil)
-                                                                                                                   pats))
-                                                       rhs GHC.Base.>>=
-                                                       (fun rhs' => GHC.Base.return_ (pair (pair dc pats) rhs')))
-                         GHC.Base.>>=
-                         (fun alts' =>
-                            GHC.Base.return_ (CoreSyn.Case (CoreSyn.deAnnotate scrut) bndr ty alts'))
-                     | captured, pair _ (CoreSyn.AnnLet ann_bind body) =>
-                         let bind := CoreSyn.deAnnBind ann_bind in
-                         let j_10__ :=
-                           go (Coq.Init.Datatypes.app captured (CoreSyn.bindersOf bind)) body GHC.Base.>>=
-                           (fun body' => GHC.Base.return_ (CoreSyn.Let bind body')) in
-                         let j_18__ :=
-                           match ann_bind with
-                           | CoreSyn.AnnRec pairs =>
-                               if Id.isJoinId (Data.Tuple.fst (GHC.List.head pairs)) : bool
-                               then let js := GHC.Base.map Data.Tuple.fst pairs in
-                                    Data.Traversable.forM pairs (fun arg_12__ =>
-                                                                   let 'pair j rhs := arg_12__ in
-                                                                   let join_arity := Id.idJoinArity j in
-                                                                   let 'pair params join_body :=
-                                                                     CoreSyn.collectNAnnBndrs join_arity rhs in
-                                                                   go (Coq.Init.Datatypes.app captured
+      GHC.DeferredFix.deferredFix2 (fun go arg_1__ arg_2__ =>
+                                      match arg_1__, arg_2__ with
+                                      | captured, ann_e =>
+                                          let j_4__ :=
+                                            match arg_1__, arg_2__ with
+                                            | _, ann_e => GHC.Base.return_ (CoreSyn.deAnnotate ann_e)
+                                            end in
+                                          let j_22__ :=
+                                            match arg_1__, arg_2__ with
+                                            | captured, pair _ (CoreSyn.AnnCase scrut bndr ty alts) =>
+                                                Data.Traversable.forM alts (fun arg_5__ =>
+                                                                              let 'pair (pair dc pats) rhs := arg_5__ in
+                                                                              go (Coq.Init.Datatypes.app captured
+                                                                                                         (Coq.Init.Datatypes.app
+                                                                                                          (cons bndr
+                                                                                                                nil)
+                                                                                                          pats)) rhs
+                                                                              GHC.Base.>>=
+                                                                              (fun rhs' =>
+                                                                                 GHC.Base.return_ (pair (pair dc pats)
+                                                                                                        rhs')))
+                                                GHC.Base.>>=
+                                                (fun alts' =>
+                                                   GHC.Base.return_ (CoreSyn.Case (CoreSyn.deAnnotate scrut) bndr ty
+                                                                                  alts'))
+                                            | captured, pair _ (CoreSyn.AnnLet ann_bind body) =>
+                                                let bind := CoreSyn.deAnnBind ann_bind in
+                                                let j_10__ :=
+                                                  go (Coq.Init.Datatypes.app captured (CoreSyn.bindersOf bind)) body
+                                                  GHC.Base.>>=
+                                                  (fun body' => GHC.Base.return_ (CoreSyn.Let bind body')) in
+                                                let j_18__ :=
+                                                  match ann_bind with
+                                                  | CoreSyn.AnnRec pairs =>
+                                                      if Id.isJoinId (Data.Tuple.fst (Panic.head pairs)) : bool
+                                                      then let js := GHC.Base.map Data.Tuple.fst pairs in
+                                                           Data.Traversable.forM pairs (fun arg_12__ =>
+                                                                                          let 'pair j rhs := arg_12__ in
+                                                                                          let join_arity :=
+                                                                                            Id.idJoinArity j in
+                                                                                          let 'pair params join_body :=
+                                                                                            CoreSyn.collectNAnnBndrs
+                                                                                              join_arity rhs in
+                                                                                          go (Coq.Init.Datatypes.app
+                                                                                              captured
                                                                                               (Coq.Init.Datatypes.app js
                                                                                                                       params))
-                                                                   join_body GHC.Base.>>=
-                                                                   (fun join_body' =>
-                                                                      let rhs' := CoreSyn.mkLams params join_body' in
-                                                                      GHC.Base.return_ (pair j rhs'))) GHC.Base.>>=
-                                    (fun pairs' =>
-                                       go (Coq.Init.Datatypes.app captured js) body GHC.Base.>>=
-                                       (fun body' => GHC.Base.return_ (CoreSyn.Let (CoreSyn.Rec pairs') body'))) else
-                               j_10__
-                           | _ => j_10__
-                           end in
-                         match ann_bind with
-                         | CoreSyn.AnnNonRec j rhs =>
-                             match Id.isJoinId_maybe j with
-                             | Some join_arity =>
-                                 let 'pair params join_body := CoreSyn.collectNAnnBndrs join_arity rhs in
-                                 go (Coq.Init.Datatypes.app captured params) join_body GHC.Base.>>=
-                                 (fun join_body' =>
-                                    let rhs' := CoreSyn.mkLams params join_body' in
-                                    go (Coq.Init.Datatypes.app captured (cons j nil)) body GHC.Base.>>=
-                                    (fun body' => GHC.Base.return_ (CoreSyn.Let (CoreSyn.NonRec j rhs') body')))
-                             | _ => j_18__
-                             end
-                         | _ => j_18__
-                         end
-                     | _, _ => j_4__
-                     end in
-                   let fvs := VarSet.dVarSetToVarSet (CoreFVs.freeVarsOf ann_e) in
-                   let e := CoreSyn.deAnnotate ann_e in
-                   let args :=
-                     GHC.List.filter (fun arg_25__ => VarSet.elemVarSet arg_25__ fvs) captured in
-                   let captures_join_points := Data.Foldable.any Id.isJoinId args in
-                   let is_interesting :=
-                     VarSet.anyVarSet Var.isLocalId (VarSet.minusVarSet fvs (VarSet.mkVarSet
-                                                                         captured)) in
-                   let isCapturedVarArg :=
-                     fun arg_29__ =>
-                       match arg_29__ with
-                       | CoreSyn.Var v => Data.Foldable.elem v captured
-                       | _ => false
-                       end in
-                   let is_exit := VarSet.disjointVarSet fvs recursive_calls in
-                   let j_36__ :=
-                     if is_exit : bool
-                     then let rhs := CoreSyn.mkLams args e in
-                          let ty := CoreUtils.exprType rhs in
-                          let avoid := VarEnv.extendInScopeSetList in_scope captured in
-                          addExit avoid ty (Data.Foldable.length args) rhs GHC.Base.>>=
-                          (fun v => GHC.Base.return_ (CoreSyn.mkVarApps (CoreSyn.Var v) args)) else
-                     j_22__ in
-                   let j_37__ :=
-                     if andb is_exit captures_join_points : bool then GHC.Base.return_ e else
-                     j_36__ in
-                   let j_38__ :=
-                     if andb is_exit (negb is_interesting) : bool then GHC.Base.return_ e else
-                     j_37__ in
-                   match CoreSyn.collectArgs e with
-                   | pair (CoreSyn.Var f) args =>
-                       if andb (Id.isJoinId f) (Data.Foldable.all isCapturedVarArg args) : bool
-                       then GHC.Base.return_ e else
-                       j_38__
-                   | _ => j_38__
-                   end
-               end in
+                                                                                          join_body GHC.Base.>>=
+                                                                                          (fun join_body' =>
+                                                                                             let rhs' :=
+                                                                                               CoreSyn.mkLams params
+                                                                                               join_body' in
+                                                                                             GHC.Base.return_ (pair j
+                                                                                                                    rhs')))
+                                                           GHC.Base.>>=
+                                                           (fun pairs' =>
+                                                              go (Coq.Init.Datatypes.app captured js) body GHC.Base.>>=
+                                                              (fun body' =>
+                                                                 GHC.Base.return_ (CoreSyn.Let (CoreSyn.Rec pairs')
+                                                                                               body'))) else
+                                                      j_10__
+                                                  | _ => j_10__
+                                                  end in
+                                                match ann_bind with
+                                                | CoreSyn.AnnNonRec j rhs =>
+                                                    match Id.isJoinId_maybe j with
+                                                    | Some join_arity =>
+                                                        let 'pair params join_body := CoreSyn.collectNAnnBndrs
+                                                                                        join_arity rhs in
+                                                        go (Coq.Init.Datatypes.app captured params) join_body
+                                                        GHC.Base.>>=
+                                                        (fun join_body' =>
+                                                           let rhs' := CoreSyn.mkLams params join_body' in
+                                                           go (Coq.Init.Datatypes.app captured (cons j nil)) body
+                                                           GHC.Base.>>=
+                                                           (fun body' =>
+                                                              GHC.Base.return_ (CoreSyn.Let (CoreSyn.NonRec j rhs')
+                                                                                            body')))
+                                                    | _ => j_18__
+                                                    end
+                                                | _ => j_18__
+                                                end
+                                            | _, _ => j_4__
+                                            end in
+                                          let fvs := VarSet.dVarSetToVarSet (CoreFVs.freeVarsOf ann_e) in
+                                          let e := CoreSyn.deAnnotate ann_e in
+                                          let args :=
+                                            GHC.List.filter (fun arg_25__ => VarSet.elemVarSet arg_25__ fvs) captured in
+                                          let captures_join_points := Data.Foldable.any Id.isJoinId args in
+                                          let is_interesting :=
+                                            VarSet.anyVarSet Var.isLocalId (VarSet.minusVarSet fvs (VarSet.mkVarSet
+                                                                                                captured)) in
+                                          let isCapturedVarArg :=
+                                            fun arg_29__ =>
+                                              match arg_29__ with
+                                              | CoreSyn.Var v => Data.Foldable.elem v captured
+                                              | _ => false
+                                              end in
+                                          let is_exit := VarSet.disjointVarSet fvs recursive_calls in
+                                          let j_35__ :=
+                                            if is_exit : bool
+                                            then let rhs := CoreSyn.mkLams args e in
+                                                 let ty := tt in
+                                                 let avoid := VarEnv.extendInScopeSetList in_scope captured in
+                                                 addExit avoid ty (Data.Foldable.length args) rhs GHC.Base.>>=
+                                                 (fun v =>
+                                                    GHC.Base.return_ (CoreSyn.mkVarApps (CoreSyn.Var v) args)) else
+                                            j_22__ in
+                                          let j_36__ :=
+                                            if andb is_exit captures_join_points : bool then GHC.Base.return_ e else
+                                            j_35__ in
+                                          let j_37__ :=
+                                            if andb is_exit (negb is_interesting) : bool then GHC.Base.return_ e else
+                                            j_36__ in
+                                          match CoreSyn.collectArgs e with
+                                          | pair (CoreSyn.Var f) args =>
+                                              if andb (Id.isJoinId f) (Data.Foldable.all isCapturedVarArg args) : bool
+                                              then GHC.Base.return_ e else
+                                              j_37__
+                                          | _ => j_37__
+                                          end
+                                      end) in
     let ann_pairs := GHC.Base.map (Data.Bifunctor.second CoreFVs.freeVars) pairs in
-    let 'pair pairs' exits := (fun arg_42__ => State.runState arg_42__ nil)
-                                (Data.Traversable.forM ann_pairs (fun arg_43__ =>
-                                                          let 'pair x rhs := arg_43__ in
+    let 'pair pairs' exits := (fun arg_41__ => State.runState arg_41__ nil)
+                                (Data.Traversable.forM ann_pairs (fun arg_42__ =>
+                                                          let 'pair x rhs := arg_42__ in
                                                           let 'pair args body := CoreSyn.collectNAnnBndrs
                                                                                    (Id.idJoinArity x) rhs in
                                                           go args body GHC.Base.>>=
                                                           (fun body' =>
                                                              let rhs' := CoreSyn.mkLams args body' in
                                                              GHC.Base.return_ (pair x rhs')))) in
-    let fix mkExitLets arg_49__
-              := match arg_49__ with
+    let fix mkExitLets arg_48__
+              := match arg_48__ with
                  | cons (pair exitId exitRhs) exits' =>
                      CoreSyn.mkLetNonRec exitId exitRhs GHC.Base.∘ mkExitLets exits'
                  | nil => GHC.Base.id
                  end in
     fun body => mkExitLets exits (CoreSyn.mkLetRec pairs' body).
 
-Definition exitifyProgram : CoreSyn.CoreProgram -> CoreSyn.CoreProgram :=
-  fun binds =>
-    let go : VarEnv.InScopeSet -> CoreSyn.CoreExpr -> CoreSyn.CoreExpr :=
-      fix go arg_0__ arg_1__
-            := match arg_0__, arg_1__ with
-               | _, (CoreSyn.Var _ as e) => e
-               | _, (CoreSyn.Lit _ as e) => e
-               | _, (CoreSyn.Type_ _ as e) => e
-               | _, (CoreSyn.Coercion _ as e) => e
-               | in_scope, CoreSyn.Lam v e' =>
-                   let in_scope' := VarEnv.extendInScopeSet in_scope v in
-                   CoreSyn.Lam v (go in_scope' e')
-               | in_scope, CoreSyn.App e1 e2 => CoreSyn.App (go in_scope e1) (go in_scope e2)
-               | in_scope, CoreSyn.Case scrut bndr ty alts =>
-                   let in_scope' := VarEnv.extendInScopeSet in_scope bndr in
-                   CoreSyn.Case (go in_scope scrut) bndr ty (GHC.Base.map (goAlt in_scope') alts)
-               | in_scope, CoreSyn.Cast e' c => CoreSyn.Cast (go in_scope e') c
-               | in_scope, CoreSyn.Tick t e' => CoreSyn.Tick t (go in_scope e')
-               | in_scope, CoreSyn.Let bind body =>
-                   let in_scope' :=
-                     VarEnv.extendInScopeSetList in_scope (CoreSyn.bindersOf bind) in
-                   goBind in_scope bind (go in_scope' body)
-               end in
-    let goAlt : VarEnv.InScopeSet -> CoreSyn.CoreAlt -> CoreSyn.CoreAlt :=
-      fun arg_12__ arg_13__ =>
-        match arg_12__, arg_13__ with
-        | in_scope, pair (pair dc pats) rhs =>
-            let in_scope' := VarEnv.extendInScopeSetList in_scope pats in
-            pair (pair dc pats) (go in_scope' rhs)
-        end in
-    let goBind
-     : VarEnv.InScopeSet ->
-       CoreSyn.CoreBind -> (CoreSyn.CoreExpr -> CoreSyn.CoreExpr) :=
-      fun arg_17__ arg_18__ =>
-        match arg_17__, arg_18__ with
-        | in_scope, CoreSyn.NonRec v rhs =>
-            CoreSyn.Let (CoreSyn.NonRec v (go in_scope rhs))
-        | in_scope, CoreSyn.Rec pairs =>
-            let in_scope' :=
-              VarEnv.extendInScopeSetList in_scope (CoreSyn.bindersOf (CoreSyn.Rec pairs)) in
-            let is_join_rec :=
-              Data.Foldable.any (Id.isJoinId GHC.Base.∘ Data.Tuple.fst) pairs in
-            let pairs' := GHC.Base.map (Data.Bifunctor.second (go in_scope')) pairs in
-            if is_join_rec : bool then exitify in_scope' pairs' else
-            CoreSyn.Let (CoreSyn.Rec pairs')
-        end in
-    let in_scope_toplvl :=
-      VarEnv.extendInScopeSetList VarEnv.emptyInScopeSet (CoreSyn.bindersOfBinds
-                                   binds) in
-    let goTopLvl :=
-      fun arg_27__ =>
-        match arg_27__ with
-        | CoreSyn.NonRec v e => CoreSyn.NonRec v (go in_scope_toplvl e)
-        | CoreSyn.Rec pairs =>
-            CoreSyn.Rec (GHC.Base.map (Data.Bifunctor.second (go in_scope_toplvl)) pairs)
-        end in
-    GHC.Base.map goTopLvl binds.
-
 (* External variables:
-     Some andb bool cons false goAlt goBind list negb nil op_zt__ pair true unit
+     Some andb bool cons false list negb nil op_zt__ pair true tt unit
      BasicTypes.AlwaysTailCalled BasicTypes.JoinArity BasicTypes.OneOcc
      Coq.Init.Datatypes.app CoreFVs.CoreExprWithFVs CoreFVs.freeVars
      CoreFVs.freeVarsOf CoreSyn.AnnCase CoreSyn.AnnLet CoreSyn.AnnNonRec
-     CoreSyn.AnnRec CoreSyn.App CoreSyn.Case CoreSyn.Cast CoreSyn.Coercion
-     CoreSyn.CoreAlt CoreSyn.CoreBind CoreSyn.CoreExpr CoreSyn.CoreProgram
-     CoreSyn.Lam CoreSyn.Let CoreSyn.Lit CoreSyn.NonRec CoreSyn.Rec CoreSyn.Tick
-     CoreSyn.Type_ CoreSyn.Var CoreSyn.bindersOf CoreSyn.bindersOfBinds
-     CoreSyn.collectArgs CoreSyn.collectNAnnBndrs CoreSyn.deAnnBind
-     CoreSyn.deAnnotate CoreSyn.mkLams CoreSyn.mkLetNonRec CoreSyn.mkLetRec
-     CoreSyn.mkVarApps CoreUtils.exprType Data.Bifunctor.second Data.Foldable.all
-     Data.Foldable.any Data.Foldable.elem Data.Foldable.length Data.Traversable.forM
-     Data.Tuple.fst FastString.fsLit GHC.Base.id GHC.Base.map GHC.Base.op_z2218U__
-     GHC.Base.op_zgzg__ GHC.Base.op_zgzgze__ GHC.Base.return_ GHC.List.filter
-     GHC.List.head Id.asJoinId Id.idJoinArity Id.isJoinId Id.isJoinId_maybe
-     Id.mkSysLocal Id.setIdOccInfo State.State State.get State.put State.runState
-     Unique.initExitJoinUnique Var.Id Var.JoinId Var.Var Var.isLocalId
-     VarEnv.InScopeSet VarEnv.emptyInScopeSet VarEnv.extendInScopeSet
+     CoreSyn.AnnRec CoreSyn.Case CoreSyn.CoreExpr CoreSyn.Let CoreSyn.NonRec
+     CoreSyn.Rec CoreSyn.Var CoreSyn.bindersOf CoreSyn.collectArgs
+     CoreSyn.collectNAnnBndrs CoreSyn.deAnnBind CoreSyn.deAnnotate CoreSyn.mkLams
+     CoreSyn.mkLetNonRec CoreSyn.mkLetRec CoreSyn.mkVarApps Data.Bifunctor.second
+     Data.Foldable.all Data.Foldable.any Data.Foldable.elem Data.Foldable.length
+     Data.Traversable.forM Data.Tuple.fst FastString.fsLit GHC.Base.id GHC.Base.map
+     GHC.Base.op_z2218U__ GHC.Base.op_zgzg__ GHC.Base.op_zgzgze__ GHC.Base.return_
+     GHC.DeferredFix.deferredFix2 GHC.List.filter Id.asJoinId Id.idJoinArity
+     Id.isJoinId Id.isJoinId_maybe Id.mkSysLocal Id.setIdOccInfo Panic.head
+     State.State State.get State.put State.runState Unique.initExitJoinUnique Var.Id
+     Var.JoinId Var.Var Var.isLocalId VarEnv.InScopeSet VarEnv.extendInScopeSet
      VarEnv.extendInScopeSetList VarEnv.uniqAway VarSet.anyVarSet
      VarSet.dVarSetToVarSet VarSet.disjointVarSet VarSet.elemVarSet
      VarSet.minusVarSet VarSet.mkVarSet
