examples/ghc/lib/Id.v
@@ -12,7 +12,7 @@ Require Coq.Program.Wf.
 
 (* Preamble *)
 
-Require Panic.
+
 
 (* Converted imports: *)
 
@@ -21,29 +21,23 @@ Require CoreSyn.
 Require DataCon.
 Require Demand.
 Require FastString.
-Require GHC.Base.
 Require GHC.Num.
 Require IdInfo.
-Require Maybes.
 Require Module.
 Require Name.
 Require OccName.
-Require Panic.
 Require SrcLoc.
 Require UniqSupply.
 Require Unique.
-Require Util.
 Require Var.
-Import GHC.Base.Notations.
-Import GHC.Num.Notations.
 
 (* No type declarations to convert. *)
 (* Midamble *)
 
 (* Record selectors *)
 Import IdInfo.
-Import IdInfo2.
 
+(*
 Parameter hasNoBinding : Var.Id -> bool.
 
 Parameter isDictId : Var.Id -> bool.
@@ -94,507 +88,252 @@ Parameter mkLocalIdOrCoVar : Name.Name -> Core.Type_ -> Var.Id.
 Parameter mkTemplateLocalsNum : GHC.Num.Int -> list Core.Type_ -> list Var.Id.
 
 Parameter setIdType : Var.Id -> Core.Type_ -> Var.Id.
-
+*)
 (* Converted value declarations: *)
 
-Definition asJoinId : Var.Id -> BasicTypes.JoinArity -> Var.JoinId :=
-  fun id arity =>
-    let is_vanilla_or_join :=
-      fun id =>
-        match Var.idDetails id with
-        | IdInfo.VanillaId => true
-        | IdInfo.JoinId _ => true
-        | _ => false
-        end in
-    Panic.warnPprTrace (negb (Var.isLocalId id)) (GHC.Base.hs_string__
-                        "ghc/compiler/basicTypes/Id.hs") #590 (GHC.Base.mappend (id
-                                                                                 (GHC.Base.hs_string__
-                                                                                  "global id being marked as join var:"))
-                                                                                (Panic.noString id)) (Panic.warnPprTrace
-                                                                                                      (negb
-                                                                                                       (is_vanilla_or_join
-                                                                                                        id))
-                                                                                                      (GHC.Base.hs_string__
-                                                                                                       "ghc/compiler/basicTypes/Id.hs")
-                                                                                                      #592
-                                                                                                      (GHC.Base.mappend
-                                                                                                       (Panic.noString
-                                                                                                        id)
-                                                                                                       (IdInfo.pprIdDetails
-                                                                                                        (Var.idDetails
-                                                                                                         id)))
-                                                                                                      (Var.setIdDetails
-                                                                                                       id (IdInfo.JoinId
-                                                                                                        arity))).
-
-Definition idArity : Var.Id -> BasicTypes.Arity :=
-  fun id => IdInfo.arityInfo (Var.idInfo id).
-
-Definition idCafInfo : Var.Id -> IdInfo.CafInfo :=
-  fun id => IdInfo.cafInfo (Var.idInfo id).
-
-Definition idCallArity : Var.Id -> BasicTypes.Arity :=
-  fun id => IdInfo.callArityInfo (Var.idInfo id).
-
-Definition idDataCon : Var.Id -> DataCon.DataCon :=
-  fun id =>
-    Maybes.orElse (isDataConId_maybe id) (Panic.panicStr (GHC.Base.hs_string__
-                                                          "idDataCon") (Panic.noString id)).
-
-Definition idDemandInfo : Var.Id -> Demand.Demand :=
-  fun id => IdInfo.demandInfo (Var.idInfo id).
-
-Definition idInlinePragma : Var.Id -> BasicTypes.InlinePragma :=
-  fun id => IdInfo.inlinePragInfo (Var.idInfo id).
-
-Definition idRuleMatchInfo : Var.Id -> BasicTypes.RuleMatchInfo :=
-  fun id => BasicTypes.inlinePragmaRuleMatchInfo (idInlinePragma id).
-
-Definition isConLikeId : Var.Id -> bool :=
-  fun id => orb (isDataConWorkId id) (BasicTypes.isConLike (idRuleMatchInfo id)).
-
-Definition idInlineActivation : Var.Id -> BasicTypes.Activation :=
-  fun id => BasicTypes.inlinePragmaActivation (idInlinePragma id).
-
-Definition idName : Var.Id -> Name.Name :=
-  Var.varName.
-
-Definition idIsFrom : Module.Module -> Var.Id -> bool :=
-  fun mod_ id => Name.nameIsLocalOrFrom mod_ (idName id).
-
-Definition idOccInfo : Var.Id -> BasicTypes.OccInfo :=
-  fun id => IdInfo.occInfo (Var.idInfo id).
-
-Definition isDeadBinder : Var.Id -> bool :=
-  fun bndr =>
-    if Var.isId bndr : bool then BasicTypes.isDeadOcc (idOccInfo bndr) else
-    false.
-
-Definition idOneShotInfo : Var.Id -> BasicTypes.OneShotInfo :=
-  fun id => IdInfo.oneShotInfo (Var.idInfo id).
-
-Definition idSpecialisation : Var.Id -> IdInfo.RuleInfo :=
-  fun id => IdInfo.ruleInfo (Var.idInfo id).
-
-Definition idHasRules : Var.Id -> bool :=
-  fun id => negb (IdInfo.isEmptyRuleInfo (idSpecialisation id)).
-
-Definition idCoreRules : Var.Id -> list CoreSyn.CoreRule :=
-  fun id => IdInfo.ruleInfoRules (idSpecialisation id).
-
-Definition idStrictness : Var.Id -> Demand.StrictSig :=
-  fun id => IdInfo.strictnessInfo (Var.idInfo id).
-
-Definition isBottomingId : Var.Var -> bool :=
-  fun v =>
-    if Var.isId v : bool then Demand.isBottomingSig (idStrictness v) else
-    false.
-
-Definition idType : Var.Id -> unit :=
-  Var.varType.
-
-Definition localiseId : Var.Id -> Var.Id :=
-  fun id =>
-    let name := idName id in
-    if (if andb Util.debugIsOn (negb (Var.isId id)) : bool
-        then (Panic.assertPanic (GHC.Base.hs_string__ "ghc/compiler/basicTypes/Id.hs")
-              #209)
-        else andb (Var.isLocalId id) (Name.isInternalName name)) : bool
-    then id else
-    Var.mkLocalVar (Var.idDetails id) (Name.localiseName name) (idType id)
-    (Var.idInfo id).
-
-Definition idFunRepArity : Var.Id -> BasicTypes.RepArity :=
-  fun x => RepType.countFunRepArgs (idArity x) (idType x).
-
-Definition idUnfolding : Var.Id -> CoreSyn.Unfolding :=
-  fun id =>
-    let info := Var.idInfo id in
-    if BasicTypes.isStrongLoopBreaker (IdInfo.occInfo info) : bool
-    then CoreSyn.NoUnfolding else
-    IdInfo.unfoldingInfo info.
-
-Definition idUnique : Var.Id -> Unique.Unique :=
-  Var.varUnique.
-
-Definition isDFunId : Var.Id -> bool :=
-  fun id =>
-    match Var.idDetails id with
-    | IdInfo.DFunId _ => true
-    | _ => false
-    end.
-
-Definition isDataConRecordSelector : Var.Id -> bool :=
-  fun id =>
-    match Var.idDetails id with
-    | IdInfo.RecSelId (IdInfo.RecSelData _) _ => true
-    | _ => false
-    end.
-
-Definition isImplicitId : Var.Id -> bool :=
-  fun id =>
-    match Var.idDetails id with
-    | IdInfo.FCallId _ => true
-    | IdInfo.ClassOpId _ => true
-    | IdInfo.PrimOpId _ => true
-    | IdInfo.DataConWorkId _ => true
-    | IdInfo.DataConWrapId _ => true
-    | _ => false
-    end.
-
-Definition isJoinId : Var.Var -> bool :=
-  fun id =>
-    if Var.isId id : bool
-    then match Var.idDetails id with
-         | IdInfo.JoinId _ => true
-         | _ => false
-         end else
-    false.
-
-Definition isExitJoinId : Var.Var -> bool :=
-  fun id =>
-    andb (isJoinId id) (andb (BasicTypes.isOneOcc (idOccInfo id))
-                             (BasicTypes.occ_in_lam (idOccInfo id))).
-
-Definition isJoinId_maybe : Var.Var -> option BasicTypes.JoinArity :=
-  fun id =>
-    if Var.isId id : bool
-    then if andb Util.debugIsOn (negb (Var.isId id)) : bool
-         then (Outputable.assertPprPanic (GHC.Base.hs_string__
-                                          "ghc/compiler/basicTypes/Id.hs") #494 (Panic.noString id))
-         else match Var.idDetails id with
-              | IdInfo.JoinId arity => Some arity
-              | _ => None
-              end else
-    None.
-
-Definition idJoinArity : Var.JoinId -> BasicTypes.JoinArity :=
-  fun id =>
-    Maybes.orElse (isJoinId_maybe id) (Panic.panicStr (GHC.Base.hs_string__
-                                                       "idJoinArity") (Panic.noString id)).
-
-Definition isNaughtyRecordSelector : Var.Id -> bool :=
-  fun id =>
-    match Var.idDetails id with
-    | IdInfo.RecSelId _ n => n
-    | _ => false
-    end.
-
-Definition isNeverLevPolyId : Var.Id -> bool :=
-  IdInfo.isNeverLevPolyIdInfo GHC.Base.∘ Var.idInfo.
-
-Definition isPatSynRecordSelector : Var.Id -> bool :=
-  fun id =>
-    match Var.idDetails id with
-    | IdInfo.RecSelId (IdInfo.RecSelPatSyn _) _ => true
-    | _ => false
-    end.
-
-Definition isRecordSelector : Var.Id -> bool :=
-  fun id =>
-    match Var.idDetails id with
-    | IdInfo.RecSelId _ _ => true
-    | _ => false
-    end.
-
-Definition lazySetIdInfo : Var.Id -> IdInfo.IdInfo -> Var.Id :=
-  Var.lazySetIdInfo.
-
-Definition maybeModifyIdInfo : option IdInfo.IdInfo -> Var.Id -> Var.Id :=
-  fun arg_0__ arg_1__ =>
-    match arg_0__, arg_1__ with
-    | Some new_info, id => lazySetIdInfo id new_info
-    | None, id => id
-    end.
-
-Definition zapInfo
-   : (IdInfo.IdInfo -> option IdInfo.IdInfo) -> Var.Id -> Var.Id :=
-  fun zapper id => maybeModifyIdInfo (zapper (Var.idInfo id)) id.
-
-Definition zapFragileIdInfo : Var.Id -> Var.Id :=
-  zapInfo IdInfo.zapFragileInfo.
-
-Definition zapIdDemandInfo : Var.Id -> Var.Id :=
-  zapInfo IdInfo.zapDemandInfo.
-
-Definition zapIdTailCallInfo : Var.Id -> Var.Id :=
-  zapInfo IdInfo.zapTailCallInfo.
-
-Definition zapJoinId : Var.Id -> Var.Id :=
-  fun jid =>
-    if isJoinId jid : bool
-    then zapIdTailCallInfo (Var.setIdDetails jid IdInfo.VanillaId) else
-    jid.
-
-Definition asJoinId_maybe : Var.Id -> option BasicTypes.JoinArity -> Var.Id :=
-  fun arg_0__ arg_1__ =>
-    match arg_0__, arg_1__ with
-    | id, Some arity => asJoinId id arity
-    | id, None => zapJoinId id
-    end.
-
-Definition zapIdUsageEnvInfo : Var.Id -> Var.Id :=
-  zapInfo IdInfo.zapUsageEnvInfo.
-
-Definition zapIdUsageInfo : Var.Id -> Var.Id :=
-  zapInfo IdInfo.zapUsageInfo.
-
-Definition zapIdUsedOnceInfo : Var.Id -> Var.Id :=
-  zapInfo IdInfo.zapUsedOnceInfo.
-
-Definition zapLamIdInfo : Var.Id -> Var.Id :=
-  zapInfo IdInfo.zapLamInfo.
-
-Definition setIdInfo : Var.Id -> IdInfo.IdInfo -> Var.Id :=
-  fun id info => lazySetIdInfo id info.
-
-Definition modifyIdInfo
-   : (IdInfo.IdInfo -> IdInfo.IdInfo) -> Var.Id -> Var.Id :=
-  fun fn id => setIdInfo id (fn (Var.idInfo id)).
-
-Definition modifyInlinePragma
-   : Var.Id -> (BasicTypes.InlinePragma -> BasicTypes.InlinePragma) -> Var.Id :=
-  fun id fn =>
-    modifyIdInfo (fun info =>
-                    IdInfo.setInlinePragInfo info (fn (IdInfo.inlinePragInfo info))) id.
-
-Definition setInlineActivation : Var.Id -> BasicTypes.Activation -> Var.Id :=
-  fun id act =>
-    modifyInlinePragma id (fun prag =>
-                             BasicTypes.setInlinePragmaActivation prag act).
-
-Definition setIdArity : Var.Id -> BasicTypes.Arity -> Var.Id :=
-  fun id arity =>
-    modifyIdInfo (fun arg_0__ => IdInfo.setArityInfo arg_0__ arity) id.
-
-Definition setIdCafInfo : Var.Id -> IdInfo.CafInfo -> Var.Id :=
-  fun id caf_info =>
-    modifyIdInfo (fun arg_0__ => IdInfo.setCafInfo arg_0__ caf_info) id.
-
-Definition setIdCallArity : Var.Id -> BasicTypes.Arity -> Var.Id :=
-  fun id arity =>
-    modifyIdInfo (fun arg_0__ => IdInfo.setCallArityInfo arg_0__ arity) id.
-
-Definition setIdDemandInfo : Var.Id -> Demand.Demand -> Var.Id :=
-  fun id dmd => modifyIdInfo (fun arg_0__ => IdInfo.setDemandInfo arg_0__ dmd) id.
-
-Definition setIdOccInfo : Var.Id -> BasicTypes.OccInfo -> Var.Id :=
-  fun id occ_info =>
-    modifyIdInfo (fun arg_0__ => IdInfo.setOccInfo arg_0__ occ_info) id.
-
-Definition zapIdOccInfo : Var.Id -> Var.Id :=
-  fun b => setIdOccInfo b BasicTypes.noOccInfo.
-
-Definition setIdOneShotInfo : Var.Id -> BasicTypes.OneShotInfo -> Var.Id :=
-  fun id one_shot =>
-    modifyIdInfo (fun arg_0__ => IdInfo.setOneShotInfo arg_0__ one_shot) id.
-
-Definition updOneShotInfo : Var.Id -> BasicTypes.OneShotInfo -> Var.Id :=
-  fun id one_shot =>
-    let do_upd :=
-      match pair (idOneShotInfo id) one_shot with
-      | pair BasicTypes.NoOneShotInfo _ => true
-      | pair BasicTypes.OneShotLam _ => false
-      end in
-    if do_upd : bool then setIdOneShotInfo id one_shot else
-    id.
-
-Definition setIdSpecialisation : Var.Id -> IdInfo.RuleInfo -> Var.Id :=
-  fun id spec_info =>
-    modifyIdInfo (fun arg_0__ => IdInfo.setRuleInfo arg_0__ spec_info) id.
-
-Definition setIdStrictness : Var.Id -> Demand.StrictSig -> Var.Id :=
-  fun id sig =>
-    modifyIdInfo (fun arg_0__ => IdInfo.setStrictnessInfo arg_0__ sig) id.
-
-Definition setIdUnfolding : Var.Id -> CoreSyn.Unfolding -> Var.Id :=
-  fun id unfolding =>
-    modifyIdInfo (fun arg_0__ => IdInfo.setUnfoldingInfo arg_0__ unfolding) id.
-
-Definition setCaseBndrEvald : DataCon.StrictnessMark -> Var.Id -> Var.Id :=
-  fun str id =>
-    if DataCon.isMarkedStrict str : bool
-    then setIdUnfolding id CoreSyn.evaldUnfolding else
-    id.
-
-Definition setInlinePragma : Var.Id -> BasicTypes.InlinePragma -> Var.Id :=
-  fun id prag =>
-    modifyIdInfo (fun arg_0__ => IdInfo.setInlinePragInfo arg_0__ prag) id.
-
-Definition setOneShotLambda : Var.Id -> Var.Id :=
-  fun id =>
-    modifyIdInfo (fun arg_0__ =>
-                    IdInfo.setOneShotInfo arg_0__ BasicTypes.OneShotLam) id.
-
-Definition transferPolyIdInfo : Var.Id -> list Var.Var -> Var.Id -> Var.Id :=
-  fun old_id abstract_wrt new_id =>
-    let old_info := Var.idInfo old_id in
-    let old_arity := IdInfo.arityInfo old_info in
-    let old_inline_prag := IdInfo.inlinePragInfo old_info in
-    let old_occ_info := IdInfo.occInfo old_info in
-    let new_occ_info := BasicTypes.zapOccTailCallInfo old_occ_info in
-    let old_strictness := IdInfo.strictnessInfo old_info in
-    let arity_increase := Util.count Var.isId abstract_wrt in
-    let new_arity := old_arity GHC.Num.+ arity_increase in
-    let new_strictness :=
-      Demand.increaseStrictSigArity arity_increase old_strictness in
-    let transfer :=
-      fun new_info =>
-        IdInfo.setStrictnessInfo (IdInfo.setOccInfo (IdInfo.setInlinePragInfo
-                                                     (IdInfo.setArityInfo new_info new_arity) old_inline_prag)
-                                                    new_occ_info) new_strictness in
-    modifyIdInfo transfer new_id.
-
-Definition zapIdStrictness : Var.Id -> Var.Id :=
-  fun id =>
-    modifyIdInfo (fun arg_0__ => IdInfo.setStrictnessInfo arg_0__ Demand.nopSig) id.
-
-Definition clearOneShotLambda : Var.Id -> Var.Id :=
-  fun id =>
-    modifyIdInfo (fun arg_0__ =>
-                    IdInfo.setOneShotInfo arg_0__ BasicTypes.NoOneShotInfo) id.
-
-Definition mkExportedLocalId
-   : IdInfo.IdDetails -> Name.Name -> unit -> Var.Id :=
-  fun details name ty =>
-    Var.mkExportedLocalVar details name ty IdInfo.vanillaIdInfo.
-
-Definition mkGlobalId
-   : IdInfo.IdDetails -> Name.Name -> unit -> IdInfo.IdInfo -> Var.Id :=
-  Var.mkGlobalVar.
-
-Definition mkSysLocalM {m} `{UniqSupply.MonadUnique m}
-   : FastString.FastString -> unit -> m Var.Id :=
-  fun fs ty =>
-    UniqSupply.getUniqueM GHC.Base.>>=
-    (fun uniq => GHC.Base.return_ (mkSysLocal fs uniq ty)).
-
-Definition mkSysLocalOrCoVar
-   : FastString.FastString -> Unique.Unique -> unit -> Var.Id :=
-  fun fs uniq ty => mkLocalIdOrCoVar (Name.mkSystemVarName uniq fs) ty.
-
-Definition mkSysLocalOrCoVarM {m} `{UniqSupply.MonadUnique m}
-   : FastString.FastString -> unit -> m Var.Id :=
-  fun fs ty =>
-    UniqSupply.getUniqueM GHC.Base.>>=
-    (fun uniq => GHC.Base.return_ (mkSysLocalOrCoVar fs uniq ty)).
-
-Definition mkTemplateLocal : GHC.Num.Int -> unit -> Var.Id :=
-  fun i ty =>
-    mkSysLocalOrCoVar (FastString.fsLit (GHC.Base.hs_string__ "v"))
-    (Unique.mkBuiltinUnique i) ty.
-
-Definition mkTemplateLocals : list unit -> list Var.Id :=
-  mkTemplateLocalsNum #1.
-
-Definition mkUserLocal
-   : OccName.OccName -> Unique.Unique -> unit -> SrcLoc.SrcSpan -> Var.Id :=
-  fun occ uniq ty loc =>
-    if andb Util.debugIsOn (negb (negb (TyCoRep.isCoercionType ty))) : bool
-    then (Panic.assertPanic (GHC.Base.hs_string__ "ghc/compiler/basicTypes/Id.hs")
-          #330)
-    else mkLocalId (Name.mkInternalName uniq occ loc) ty.
-
-Definition mkUserLocalOrCoVar
-   : OccName.OccName -> Unique.Unique -> unit -> SrcLoc.SrcSpan -> Var.Id :=
-  fun occ uniq ty loc => mkLocalIdOrCoVar (Name.mkInternalName uniq occ loc) ty.
-
-Definition mkWorkerId : Unique.Unique -> Var.Id -> unit -> Var.Id :=
-  fun uniq unwrkr ty =>
-    mkLocalIdOrCoVar (Name.mkDerivedInternalName OccName.mkWorkerOcc uniq
-                      (Name.getName unwrkr)) ty.
-
-Definition realIdUnfolding : Var.Id -> CoreSyn.Unfolding :=
-  fun id => IdInfo.unfoldingInfo (Var.idInfo id).
-
-Definition zapStableUnfolding : Var.Id -> Var.Id :=
-  fun id =>
-    if CoreSyn.isStableUnfolding (realIdUnfolding id) : bool
-    then setIdUnfolding id CoreSyn.NoUnfolding else
-    id.
-
-Definition recordSelectorTyCon : Var.Id -> IdInfo.RecSelParent :=
-  fun id =>
-    match Var.idDetails id with
-    | IdInfo.RecSelId parent _ => parent
-    | _ => Panic.panic (GHC.Base.hs_string__ "recordSelectorTyCon")
-    end.
-
-Definition setIdExported : Var.Id -> Var.Id :=
-  Var.setIdExported.
-
-Definition setIdName : Var.Id -> Name.Name -> Var.Id :=
-  Var.setVarName.
-
-Definition setIdNotExported : Var.Id -> Var.Id :=
-  Var.setIdNotExported.
-
-Definition setIdUnique : Var.Id -> Unique.Unique -> Var.Id :=
-  Var.setVarUnique.
-
-Definition stateHackOneShot : BasicTypes.OneShotInfo :=
-  BasicTypes.OneShotLam.
-
-Definition idStateHackOneShotInfo : Var.Id -> BasicTypes.OneShotInfo :=
-  fun id =>
-    if isStateHackType (idType id) : bool then stateHackOneShot else
-    idOneShotInfo id.
-
-Definition isOneShotBndr : Var.Var -> bool :=
-  fun var =>
-    if Var.isTyVar var : bool then true else
-    match idStateHackOneShotInfo var with
-    | BasicTypes.OneShotLam => true
-    | _ => false
-    end.
-
-Definition isProbablyOneShotLambda : Var.Id -> bool :=
-  fun id =>
-    match idStateHackOneShotInfo id with
-    | BasicTypes.OneShotLam => true
-    | BasicTypes.NoOneShotInfo => false
-    end.
+Axiom idIsFrom : Module.Module -> Var.Id -> bool.
+
+Axiom localiseId : Var.Id -> Var.Id.
+
+Axiom idName : Var.Id -> Name.Name.
+
+Axiom idUnique : Var.Id -> Unique.Unique.
+
+Axiom isProbablyOneShotLambda : Var.Id -> bool.
+
+Axiom isOneShotBndr : Var.Var -> bool.
+
+Axiom idStateHackOneShotInfo : Var.Id -> BasicTypes.OneShotInfo.
+
+(* isStrictId skipped *)
+
+Axiom idFunRepArity : Var.Id -> BasicTypes.RepArity.
+
+(* isDictId skipped *)
+
+Axiom idType : Var.Id -> unit.
+
+Axiom setIdName : Var.Id -> Name.Name -> Var.Id.
+
+Axiom setIdUnique : Var.Id -> Unique.Unique -> Var.Id.
+
+(* setIdType skipped *)
+
+Axiom setIdExported : Var.Id -> Var.Id.
+
+Axiom setIdNotExported : Var.Id -> Var.Id.
+
+Axiom asJoinId_maybe : Var.Id -> option BasicTypes.JoinArity -> Var.Id.
+
+Axiom zapJoinId : Var.Id -> Var.Id.
+
+Axiom zapIdTailCallInfo : Var.Id -> Var.Id.
+
+Axiom zapIdUsedOnceInfo : Var.Id -> Var.Id.
+
+Axiom zapIdUsageEnvInfo : Var.Id -> Var.Id.
+
+Axiom zapIdUsageInfo : Var.Id -> Var.Id.
+
+Axiom zapIdDemandInfo : Var.Id -> Var.Id.
+
+Axiom zapFragileIdInfo : Var.Id -> Var.Id.
+
+Axiom zapLamIdInfo : Var.Id -> Var.Id.
+
+Axiom zapInfo : (IdInfo.IdInfo -> option IdInfo.IdInfo) -> Var.Id -> Var.Id.
+
+Axiom maybeModifyIdInfo : option IdInfo.IdInfo -> Var.Id -> Var.Id.
+
+Axiom transferPolyIdInfo : Var.Id -> list Var.Var -> Var.Id -> Var.Id.
+
+Axiom updOneShotInfo : Var.Id -> BasicTypes.OneShotInfo -> Var.Id.
+
+Axiom setIdOneShotInfo : Var.Id -> BasicTypes.OneShotInfo -> Var.Id.
+
+Axiom clearOneShotLambda : Var.Id -> Var.Id.
+
+Axiom setOneShotLambda : Var.Id -> Var.Id.
+
+Axiom setInlineActivation : Var.Id -> BasicTypes.Activation -> Var.Id.
+
+Axiom modifyInlinePragma : Var.Id ->
+                           (BasicTypes.InlinePragma -> BasicTypes.InlinePragma) -> Var.Id.
+
+Axiom setInlinePragma : Var.Id -> BasicTypes.InlinePragma -> Var.Id.
+
+Axiom zapIdOccInfo : Var.Id -> Var.Id.
+
+Axiom setIdOccInfo : Var.Id -> BasicTypes.OccInfo -> Var.Id.
+
+Axiom setIdCafInfo : Var.Id -> IdInfo.CafInfo -> Var.Id.
+
+Axiom setIdSpecialisation : Var.Id -> IdInfo.RuleInfo -> Var.Id.
+
+Axiom setIdDemandInfo : Var.Id -> Demand.Demand -> Var.Id.
+
+Axiom zapStableUnfolding : Var.Id -> Var.Id.
+
+Axiom setCaseBndrEvald : DataCon.StrictnessMark -> Var.Id -> Var.Id.
+
+Axiom setIdUnfolding : Var.Id -> CoreSyn.Unfolding -> Var.Id.
+
+Axiom zapIdStrictness : Var.Id -> Var.Id.
+
+Axiom setIdStrictness : Var.Id -> Demand.StrictSig -> Var.Id.
+
+Axiom setIdCallArity : Var.Id -> BasicTypes.Arity -> Var.Id.
+
+Axiom setIdArity : Var.Id -> BasicTypes.Arity -> Var.Id.
+
+Axiom modifyIdInfo : (IdInfo.IdInfo -> IdInfo.IdInfo) -> Var.Id -> Var.Id.
+
+Axiom setIdInfo : Var.Id -> IdInfo.IdInfo -> Var.Id.
+
+Axiom lazySetIdInfo : Var.Id -> IdInfo.IdInfo -> Var.Id.
+
+(* mkVanillaGlobal skipped *)
+
+(* mkVanillaGlobalWithInfo skipped *)
+
+Axiom mkGlobalId : IdInfo.IdDetails ->
+                   Name.Name -> unit -> IdInfo.IdInfo -> Var.Id.
+
+Axiom mkUserLocal : OccName.OccName ->
+                    Unique.Unique -> unit -> SrcLoc.SrcSpan -> Var.Id.
+
+Axiom mkSysLocalM : forall {m},
+                    forall `{UniqSupply.MonadUnique m}, FastString.FastString -> unit -> m Var.Id.
+
+Axiom mkSysLocal : FastString.FastString -> Unique.Unique -> unit -> Var.Id.
+
+Axiom mkWorkerId : Unique.Unique -> Var.Id -> unit -> Var.Id.
+
+Axiom mkUserLocalOrCoVar : OccName.OccName ->
+                           Unique.Unique -> unit -> SrcLoc.SrcSpan -> Var.Id.
+
+Axiom mkTemplateLocals : list unit -> list Var.Id.
+
+(* mkTemplateLocalsNum skipped *)
+
+Axiom mkTemplateLocal : GHC.Num.Int -> unit -> Var.Id.
+
+Axiom mkSysLocalOrCoVarM : forall {m},
+                           forall `{UniqSupply.MonadUnique m}, FastString.FastString -> unit -> m Var.Id.
+
+Axiom mkSysLocalOrCoVar : FastString.FastString ->
+                          Unique.Unique -> unit -> Var.Id.
+
+(* mkLocalIdOrCoVar skipped *)
+
+(* mkLocalId skipped *)
+
+(* mkLocalCoVar skipped *)
+
+(* mkLocalIdOrCoVarWithInfo skipped *)
+
+(* mkLocalIdWithInfo skipped *)
+
+Axiom mkExportedLocalId : IdInfo.IdDetails -> Name.Name -> unit -> Var.Id.
+
+(* mkExportedVanillaId skipped *)
+
+Axiom recordSelectorTyCon : Var.Id -> IdInfo.RecSelParent.
+
+Axiom isRecordSelector : Var.Id -> bool.
+
+Axiom isDataConRecordSelector : Var.Id -> bool.
+
+Axiom isPatSynRecordSelector : Var.Id -> bool.
+
+Axiom isNaughtyRecordSelector : Var.Id -> bool.
+
+(* isClassOpId_maybe skipped *)
+
+(* isPrimOpId skipped *)
+
+Axiom isDFunId : Var.Id -> bool.
+
+(* isPrimOpId_maybe skipped *)
+
+(* isFCallId skipped *)
+
+(* isFCallId_maybe skipped *)
+
+(* isConLikeId skipped *)
+
+(* isDataConWorkId skipped *)
+
+(* isDataConWorkId_maybe skipped *)
+
+(* idDataCon skipped *)
+
+(* isDataConId_maybe skipped *)
+
+Axiom isExitJoinId : Var.Var -> bool.
+
+Axiom isJoinId : Var.Var -> bool.
+
+Axiom idJoinArity : Var.JoinId -> BasicTypes.JoinArity.
+
+Axiom isJoinId_maybe : Var.Var -> option BasicTypes.JoinArity.
+
+(* hasNoBinding skipped *)
+
+Axiom isImplicitId : Var.Id -> bool.
+
+(* isDeadBinder skipped *)
+
+(* isEvVar skipped *)
+
+Axiom asJoinId : Var.Id -> BasicTypes.JoinArity -> Var.JoinId.
+
+(* idArity skipped *)
+
+(* idCallArity skipped *)
+
+(* isBottomingId skipped *)
+
+(* idStrictness skipped *)
+
+Axiom idUnfolding : Var.Id -> CoreSyn.Unfolding.
+
+Axiom realIdUnfolding : Var.Id -> CoreSyn.Unfolding.
+
+(* idDemandInfo skipped *)
+
+(* idHasRules skipped *)
+
+(* idCoreRules skipped *)
+
+(* idSpecialisation skipped *)
+
+(* idCafInfo skipped *)
+
+(* idOccInfo skipped *)
+
+(* idRuleMatchInfo skipped *)
+
+(* idInlineActivation skipped *)
+
+(* idInlinePragma skipped *)
+
+(* idOneShotInfo skipped *)
+
+(* typeOneShot skipped *)
+
+Axiom stateHackOneShot : BasicTypes.OneShotInfo.
+
+(* isStateHackType skipped *)
+
+Axiom isNeverLevPolyId : Var.Id -> bool.
 
 (* External variables:
-     None Some andb bool false isDataConId_maybe isDataConWorkId isStateHackType list
-     mkLocalId mkLocalIdOrCoVar mkSysLocal mkTemplateLocalsNum negb option orb pair
-     true unit BasicTypes.Activation BasicTypes.Arity BasicTypes.InlinePragma
-     BasicTypes.JoinArity BasicTypes.NoOneShotInfo BasicTypes.OccInfo
-     BasicTypes.OneShotInfo BasicTypes.OneShotLam BasicTypes.RepArity
-     BasicTypes.RuleMatchInfo BasicTypes.inlinePragmaActivation
-     BasicTypes.inlinePragmaRuleMatchInfo BasicTypes.isConLike BasicTypes.isDeadOcc
-     BasicTypes.isOneOcc BasicTypes.isStrongLoopBreaker BasicTypes.noOccInfo
-     BasicTypes.occ_in_lam BasicTypes.setInlinePragmaActivation
-     BasicTypes.zapOccTailCallInfo CoreSyn.CoreRule CoreSyn.NoUnfolding
-     CoreSyn.Unfolding CoreSyn.evaldUnfolding CoreSyn.isStableUnfolding
-     DataCon.DataCon DataCon.StrictnessMark DataCon.isMarkedStrict Demand.Demand
-     Demand.StrictSig Demand.increaseStrictSigArity Demand.isBottomingSig
-     Demand.nopSig FastString.FastString FastString.fsLit GHC.Base.mappend
-     GHC.Base.op_z2218U__ GHC.Base.op_zgzgze__ GHC.Base.return_ GHC.Num.Int
-     GHC.Num.fromInteger GHC.Num.op_zp__ IdInfo.CafInfo IdInfo.ClassOpId
-     IdInfo.DFunId IdInfo.DataConWorkId IdInfo.DataConWrapId IdInfo.FCallId
-     IdInfo.IdDetails IdInfo.IdInfo IdInfo.JoinId IdInfo.PrimOpId IdInfo.RecSelData
-     IdInfo.RecSelId IdInfo.RecSelParent IdInfo.RecSelPatSyn IdInfo.RuleInfo
-     IdInfo.VanillaId IdInfo.arityInfo IdInfo.cafInfo IdInfo.callArityInfo
-     IdInfo.demandInfo IdInfo.inlinePragInfo IdInfo.isEmptyRuleInfo
-     IdInfo.isNeverLevPolyIdInfo IdInfo.occInfo IdInfo.oneShotInfo
-     IdInfo.pprIdDetails IdInfo.ruleInfo IdInfo.ruleInfoRules IdInfo.setArityInfo
-     IdInfo.setCafInfo IdInfo.setCallArityInfo IdInfo.setDemandInfo
-     IdInfo.setInlinePragInfo IdInfo.setOccInfo IdInfo.setOneShotInfo
-     IdInfo.setRuleInfo IdInfo.setStrictnessInfo IdInfo.setUnfoldingInfo
-     IdInfo.strictnessInfo IdInfo.unfoldingInfo IdInfo.vanillaIdInfo
-     IdInfo.zapDemandInfo IdInfo.zapFragileInfo IdInfo.zapLamInfo
-     IdInfo.zapTailCallInfo IdInfo.zapUsageEnvInfo IdInfo.zapUsageInfo
-     IdInfo.zapUsedOnceInfo Maybes.orElse Module.Module Name.Name Name.getName
-     Name.isInternalName Name.localiseName Name.mkDerivedInternalName
-     Name.mkInternalName Name.mkSystemVarName Name.nameIsLocalOrFrom OccName.OccName
-     OccName.mkWorkerOcc Outputable.assertPprPanic Panic.assertPanic Panic.noString
-     Panic.panic Panic.panicStr Panic.warnPprTrace RepType.countFunRepArgs
-     SrcLoc.SrcSpan TyCoRep.isCoercionType UniqSupply.MonadUnique
-     UniqSupply.getUniqueM Unique.Unique Unique.mkBuiltinUnique Util.count
-     Util.debugIsOn Var.Id Var.JoinId Var.Var Var.idDetails Var.idInfo Var.isId
-     Var.isLocalId Var.isTyVar Var.lazySetIdInfo Var.mkExportedLocalVar
-     Var.mkGlobalVar Var.mkLocalVar Var.setIdDetails Var.setIdExported
-     Var.setIdNotExported Var.setVarName Var.setVarUnique Var.varName Var.varType
-     Var.varUnique
+     bool list option unit BasicTypes.Activation BasicTypes.Arity
+     BasicTypes.InlinePragma BasicTypes.JoinArity BasicTypes.OccInfo
+     BasicTypes.OneShotInfo BasicTypes.RepArity CoreSyn.Unfolding
+     DataCon.StrictnessMark Demand.Demand Demand.StrictSig FastString.FastString
+     GHC.Num.Int IdInfo.CafInfo IdInfo.IdDetails IdInfo.IdInfo IdInfo.RecSelParent
+     IdInfo.RuleInfo Module.Module Name.Name OccName.OccName SrcLoc.SrcSpan
+     UniqSupply.MonadUnique Unique.Unique Var.Id Var.JoinId Var.Var
 *)
