examples/ghc/manual/Panic.v
@@ -2,24 +2,7 @@ Require Import  GHC.Base.
 Require Import GHC.Num.
 Require Import GHC.Err.
 
-(*
-Class Default (a :Type) := {
-  default : a
-}.
-
-Instance default_num {a} `{ Num a} : Default a := { default := #0 }.
-Instance default_bool : Default bool := { default := false }.
-Instance default_monoid {a} `{ Monoid a } : Default a :=
-  { default := mempty }.
-Instance default_applicative {a}{f} `{Default a} `{Applicative f}
-  : Default (f a ) := { default := pure default }.
-
-
-Instance default_arr {a}{b} `{Default b} : Default (a -> b) :=
-  { default := fun x => default }.
-Instance default_option {a} : Default (option a) := { default := None }.
-Instance default_list {a} : Default (list a) := { default := nil } .
-*)
+Parameter head : forall {a} `{Default a}, list a -> a.
 
 Parameter noString : forall {a}, a -> String.
 Parameter someSDoc : String.
