examples/ghc/module-edits/CoreFVs/preamble.v
@@ -1,1 +1,1 @@
-
+Require Import CoreSyn.
