examples/ghc/module-edits/Id/preamble.v
@@ -1,1 +1,1 @@
-Require Panic.
+
